coq-proof/FieldDefs.v
@@ -1,0 +1,138 @@
+Require Import TacticalLemmas.
+Require Import UnitsDefs.
+Require Import SubtypingDefs.
+Require Import IDDefs.
+Require Import ValueDefs.
+Require Import GammaDefs.
+Require Import HeapDefs.
+Require Import GammaHeapCorrespondence.
+
+(* ======================================================= *)
+Inductive Field_Declarations : Type :=
+  | FD_Empty : Field_Declarations
+  | FD_Decl : Unit -> ID -> nat -> Field_Declarations -> Field_Declarations.
+Tactic Notation "fds_cases" tactic(first) ident(c) :=
+  first;
+  [ Case_aux c "FD_Empty"
+  | Case_aux c "FD_Decl"
+  ].
+Hint Constructors Field_Declarations.
+
+(* ======================================================= *)
+Reserved Notation "'fds:' g1 '|-' fds 'in' g2" (at level 40).
+Inductive fds_has_type : Gamma -> Field_Declarations -> Gamma -> Prop :=
+  | T_FD_Empty : forall (g : Gamma),
+    fds: g |- FD_Empty in g
+  | T_FD : forall (g1 g2 : Gamma) (tail : Field_Declarations) (T : Unit) (f : ID) (z : nat),
+    Gamma_Contains g1 f = false ->
+    Gamma_Contains g2 f = true ->
+    Gamma_Get g2 f = Some T ->
+    fds: Gamma_Extend g1 f T |- tail in g2 ->
+    fds: g1 |- FD_Decl T f z tail in g2
+where "'fds:' g1 '|-' fds 'in' g2" := (fds_has_type g1 fds g2).
+Tactic Notation "fds_has_type_cases" tactic(first) ident(c) :=
+  first;
+  [ Case_aux c "T_FD_Empty"
+  | Case_aux c "T_FD"
+  ].
+Hint Constructors fds_has_type.
+
+(* ======================================================= *)
+Reserved Notation " fds1 'fds==>' fds2 " (at level 8).
+Inductive fds_small_step : prod Heap Field_Declarations -> prod Heap Field_Declarations -> Prop :=
+  | ST_FD : forall (h : Heap) (T : Unit) (f : ID) (z : nat) (fds : Field_Declarations),
+    ( h, FD_Decl T f z fds ) fds==> ( (Heap_Update h f T T z), fds )
+where " fds1 'fds==>' fds2 " := (fds_small_step fds1 fds2).
+Tactic Notation "fds_small_step_cases" tactic(first) ident(c) :=
+  first;
+  [ Case_aux c "ST_FD"
+  ].
+Hint Constructors fds_small_step.
+
+(* ======================================================= *)
+(* step is deterministic *)
+Theorem fds_small_step_deterministic:
+  forall fds fds1 fds2,
+    fds fds==> fds1 ->
+    fds fds==> fds2 ->
+    fds1 = fds2.
+Proof.
+  intros fds fds1 fds2 Hfds1.
+  generalize dependent fds2.
+  fds_small_step_cases (induction Hfds1) Case.
+  Case "ST_FD".
+    intros fds2 Hfds2.
+    inversion Hfds2; subst. reflexivity.
+Qed.
+
+(* ======================================================= *)
+Inductive FD_Normal_Form : Field_Declarations -> Prop :=
+  | V_FD_Empty : FD_Normal_Form FD_Empty.
+
+(* ======================================================= *)
+Theorem fds_progress : forall (fds : Field_Declarations) (g1 g2 : Gamma) (h : Heap),
+  fds: g1 |- fds in g2 ->
+  FD_Normal_Form fds \/ exists h' fds', (h, fds) fds==> (h', fds').
+Proof.
+  (* by induction on typing of fds *)
+  intros fds g1 g2 h HT.
+  fds_has_type_cases (induction HT) Case; subst.
+  Case "T_FD_Empty".
+    left. apply V_FD_Empty.
+  Case "T_FD".
+    right.
+    destruct IHHT.
+      inversion H2. exists (Heap_Update h f T T z). exists FD_Empty. apply ST_FD.
+      exists (Heap_Update h f T T z). exists tail. apply ST_FD.
+Qed.
+
+(* ======================================================= *)
+
+(* Returns the first field definition in the list of field definitions fds, or None if the list is empty *)
+Definition First_FD (fds : Field_Declarations) : option (prod (prod Unit ID) nat) :=
+  match fds with
+  | FD_Decl T f z fds => Some (T, f, z)
+  | FD_Empty => None
+  end.
+
+(* ======================================================= *)
+
+Theorem fds_preservation : forall (g1 g2 : Gamma) (h h' : Heap) (fds fds' : Field_Declarations) (T : Unit) (f : ID) (z : nat),
+  fds: g1 |- fds in g2 ->
+  gh: g2 |- h OK ->
+  (h, fds) fds==> (h', fds') ->
+  First_FD fds = Some (T, f, z) ->
+  gh: g2 |- h' OK /\ fds: Gamma_Extend g1 f T |- fds' in g2.
+Proof.
+  intros g1 g2 h h' fds fds' T f z HT HGH HS Hfst.
+  generalize dependent fds'. generalize dependent h'.
+  fds_has_type_cases (induction HT) Case; intros h' fds' HS; subst.
+  Case "T_FD_Empty".
+    inversion HS.
+  Case "T_FD".
+    inversion HS; subst.
+    inversion Hfst; subst.
+    split.
+    (* first prove that g2 |- h' OK *)
+      apply GH_Correspondence.
+      intros f'.
+      inversion HGH; subst.
+      destruct H2 with f'. destruct H4 as [Tf']. destruct H4 as [Tv']. destruct H4 as [z'].
+        destruct H4. destruct H5. destruct H6.
+      split. apply H3.
+      destruct (id_eq_dec f' f).
+      (* Case: f = f' : in h', the value of f' is T T z *)
+        exists T, T, z.
+        rewrite -> e in H4. assert (T = Tf'). eapply Gamma_Get_Content_Eq. apply H1. apply H4. subst.
+        split. apply H1.
+        split. apply Heap_Update_FieldType_Eq.
+        split. apply subtype_reflexive.
+        apply Heap_Update_FieldValue_Eq.
+      (* Case: f <> f' : in h' the value of f' is some Tv' z' *)
+        exists Tf', Tv', z'.
+        split. apply H4.
+        split. rewrite <- H5. apply Heap_Update_FieldType_Neq. apply n.
+        split. apply H6. rewrite <- H7. apply Heap_Update_FieldValue_Neq. apply n.
+    (* then prove that fds: Gamma_Extend g1 f T |- fds' in g2 *)
+      apply HT.
+Qed.
