coq-proof/ProgramDefs.v
@@ -16,28 +16,28 @@ Require Import ValueDefs.
 Require Import GammaDefs.
 Require Import HeapDefs.
 Require Import GammaHeapCorrespondence.
-Require Import FieldsDefs.
-Require Import ExpressionsDefs.
+Require Import FieldDefs.
+Require Import ExpressionDefs.
 Require Import StatementDefs.
 
 (* ======================================================= *)
 Inductive Program : Type :=
-  | program : Field_Declaration -> Statement -> Program.
+  | program : Field_Declarations -> Statements -> Program.
 Tactic Notation "prog_cases" tactic(first) ident(c) :=
   first;
   [ Case_aux c "program"
   ].
 Hint Constructors Program.
 
-Notation "{ fd s }" := (program fd s) (at level 1).
+Notation "{ fds s }" := (program fds s) (at level 1).
 
 (* ======================================================= *)
 Reserved Notation "'prog:' g '|-' p 'in' post_gamma" (at level 40).
 Inductive prog_has_type : Gamma -> Program -> Gamma -> Prop :=
-  | T_Program : forall (g post_gamma : Gamma) (fd : Field_Declaration) (s : Statement),
-    fd: g |- fd in post_gamma ->
+  | T_Program : forall (g post_gamma : Gamma) (fds : Field_Declarations) (s : Statements),
+    fds: g |- fds in post_gamma ->
     stmt: post_gamma |- s ->
-    prog: g |- program fd s in post_gamma
+    prog: g |- program fds s in post_gamma
 where "'prog:' g '|-' p 'in' post_gamma" := (prog_has_type g p post_gamma).
 Tactic Notation "prog_has_type_cases" tactic(first) ident(c) :=
   first;
@@ -48,17 +48,17 @@ Hint Constructors prog_has_type.
 (* ======================================================= *)
 Reserved Notation " p1 'prog==>' p2 " (at level 8).
 Inductive prog_small_step : prod Heap Program -> prod Heap Program -> Prop :=
-  | ST_PROG_FieldDefs_Step : forall h h' fd fd' s,
-    ( h, fd ) fd==> ( h', fd' ) ->
-    ( h, program fd s ) prog==> ( h', program fd' s )
-  | ST_PROG_Statements_Step : forall h h' s s',
+  | ST_PROG_FieldDefs_Step : forall h h' fds fds' s,
+    ( h, fds ) fds==> ( h', fds' ) ->
+    ( h, program fds s ) prog==> ( h', program fds' s )
+  | ST_PROG_Statementss_Step : forall h h' s s',
     ( h, s ) stmt==> ( h', s' ) ->
     ( h, program FD_Empty s ) prog==> ( h', program FD_Empty s' )
 where " p1 'prog==>' p2 " := (prog_small_step p1 p2).
 Tactic Notation "prog_small_step_cases" tactic(first) ident(c) :=
   first;
   [ Case_aux c "ST_PROG_FieldDefs_Step"
-  | Case_aux c "ST_PROG_Statements_Step"
+  | Case_aux c "ST_PROG_Statementss_Step"
   ].
 Hint Constructors prog_small_step.
 
@@ -75,10 +75,10 @@ Proof.
   prog_small_step_cases (induction Hp1) Case.
   Case "ST_PROG_FieldDefs_Step".
     intros p2 Hp2; inversion Hp2; subst.
-      assert ((h', fd') = (h'0, fd'0)) as HfdEQ. eapply fd_small_step_deterministic.
-        apply H. apply H4. inversion HfdEQ; subst. reflexivity.
+      assert ((h', fds') = (h'0, fds'0)) as HfdsEQ. eapply fds_small_step_deterministic.
+        apply H. apply H4. inversion HfdsEQ; subst. reflexivity.
       inversion H.
-  Case "ST_PROG_Statements_Step".
+  Case "ST_PROG_Statementss_Step".
     intros p2 Hp2; inversion Hp2; subst.
       inversion H4.
       assert ((h', s') = (h'0, s'0)) as HsEQ. eapply stmt_small_step_deterministic.
@@ -99,9 +99,9 @@ Proof.
   intros g1 g2 p h HT HGH.
   prog_has_type_cases (induction HT) Case; subst.
   Case "T_Program".
-    assert (FD_Normal_Form fd \/ exists heap' fd', (h, fd) fd==> (heap', fd')).
-      eapply fd_progress. apply H.
-    assert (STMT_Normal_Form s \/ exists (h' : Heap) (s' : Statement), (h, s) stmt==> (h', s')).
+    assert (FD_Normal_Form fds \/ exists heap' fds', (h, fds) fds==> (heap', fds')).
+      eapply fds_progress. apply H.
+    assert (STMT_Normal_Form s \/ exists (h' : Heap) (s' : Statements), (h, s) stmt==> (h', s')).
       eapply stmt_progress. apply H0. apply HGH.
     destruct H1; subst.
     (* Case : FD is normal form *)
@@ -111,10 +111,10 @@ Proof.
       (* Case : STMT can take a step *)
         destruct H1; subst. right. destruct H2 as [h']. destruct H1 as [s'].
         exists h'. exists (program FD_Empty s').
-        apply ST_PROG_Statements_Step. apply H1.
+        apply ST_PROG_Statementss_Step. apply H1.
     (* Case : FD can take a step *)
-      destruct H1 as [h']. destruct H1 as [fd']. right.
-      exists h'. exists (program fd' s).
+      destruct H1 as [h']. destruct H1 as [fds']. right.
+      exists h'. exists (program fds' s).
       apply ST_PROG_FieldDefs_Step. apply H1.
 Qed.
 
@@ -122,7 +122,7 @@ Qed.
 
 Definition Gamma_Extend_Prog (g : Gamma) (p : Program) : Gamma :=
   match p with
-  | program fd s => match First_FD fd with
+  | program fds s => match First_FD fds with
                     | Some (T, f, z) => Gamma_Extend g f T
                     | None => g
                     end
@@ -142,12 +142,12 @@ Proof.
   generalize dependent p'. generalize dependent h'.
   prog_has_type_cases (induction HT) Case; intros h' p' HS; subst.
   Case "T_Program".
-    destruct p' as [fd' s'].
+    destruct p' as [fds' s'].
     prog_small_step_cases (inversion HS) SCase; subst.
     SCase "ST_PROG_FieldDefs_Step".
       inversion H2; subst.
       unfold Gamma_Extend_Prog. simpl.
-      eapply fd_preservation in H.
+      eapply fds_preservation in H.
       destruct H.
         split.
         (* first prove that post_gamma |- h' OK *)
@@ -159,7 +159,7 @@ Proof.
         apply HGH.
         apply H2.
         simpl. reflexivity.
-    SCase "ST_PROG_Statements_Step".
+    SCase "ST_PROG_Statementss_Step".
       simpl. (* in statement step, the input gamma to type p' does not change *)
         eapply stmt_preservation in H0.
         split.
